go/heap/struct.go
@@ -1,0 +1,56 @@
+package heap
+
+type Person struct {
+	FirstName string
+	LastName  string
+	Age       uint64
+}
+
+func (p Person) Name() string {
+	return p.FirstName + " " + p.LastName
+}
+
+func (p *Person) Older(delta uint64) {
+	p.Age += delta
+}
+
+func (p *Person) GetAge() *uint64 {
+	return &p.Age
+}
+
+func ExamplePerson() Person {
+	return Person{
+		FirstName: "Ada",
+		LastName:  "Lovelace",
+		Age:       25,
+	}
+}
+
+func ExamplePersonRef() *Person {
+	return &Person{
+		FirstName: "Ada",
+		LastName:  "Lovelace",
+		Age:       25,
+	}
+}
+
+func (p Person) BuggySetAge() {
+	p.Age += 1
+}
+
+type Rect struct {
+	Width  uint64
+	Height uint64
+}
+
+func (r Rect) Area() uint64 {
+	return r.Width * r.Height
+}
+
+func (r Rect) IsSquare() bool {
+	return r.Width == r.Height
+}
+
+func (r *Rect) MakeSquare() {
+	r.Height = r.Width
+}
